Test suite for array primitives in pulse. Beginning of an insertion sort implementation in pulse

share/steel/examples/pulse/ArrayTests.fst
@@ -3,6 +3,7 @@ module T = FStar.Tactics
 module PM = Pulse.Main
 open Steel.ST.Util 
 open Steel.ST.Array
+open Steel.ST.Reference
 open Steel.FractionalPermission
 open FStar.Ghost
 module U32 = FStar.UInt32
@@ -79,58 +80,6 @@ fn read_at_offset (a:array U32.t) (i:US.t) (#p:perm) (#s:Ghost.erased (Seq.seq U
 } 
 ```
 
-assume
-val test_array_access
-  (#t: Type)
-  (a: A.array t)
-  (i: US.t)
-  (#s: Ghost.erased (Seq.seq t) {US.v i < A.length a \/ US.v i < Seq.length s})
-  (#p: perm)
-: stt t
-    (requires
-      A.pts_to a p s)
-    (ensures fun res ->
-      A.pts_to a p s `star`
-      pure (Seq.length s == A.length a /\
-            US.v i < Seq.length s /\
-            res == Seq.index s (US.v i)))
-
-```pulse
-fn read_at_offset_refine (a:array U32.t) (i:US.t) (#p:perm) (#s:Ghost.erased (Seq.seq U32.t))
-   requires (A.pts_to a p s `star`
-             pure (US.v i < A.length a \/ US.v i < Seq.length s))
-   returns x:U32.t
-   ensures (
-      A.pts_to a p s
-     `star`
-      pure (Seq.length s == A.length a /\
-            US.v i < Seq.length s /\
-            x == Seq.index s (US.v i))
-   )
-{ 
-   let x = test_array_access a i;
-   x
-} 
-```
-
-
-```pulse
-fn read_at_offset_refine_poly (#t:Type0) (a:array t) (i:US.t) (#p:perm) (#s:Ghost.erased (Seq.seq t))
-   requires (A.pts_to a p s `star`
-             pure (US.v i < A.length a \/ US.v i < Seq.length s))
-   returns x:t
-   ensures (
-      A.pts_to a p s
-     `star`
-      pure (Seq.length s == A.length a /\
-            US.v i < Seq.length s /\
-            x == Seq.index s (US.v i))
-   )
-{ 
-   let x = test_array_access a i;
-   x
-} 
-```
 //Error message is poor as usual
 //But, this type is genuinely incorrect, since the return type does not assume
 //the validity of the pure conjuncts in the requires
@@ -139,7 +88,7 @@ fn read_at_offset_refine_poly (#t:Type0) (a:array t) (i:US.t) (#p:perm) (#s:Ghos
 //Megan correctly remarks that this is unintuitive ... let's see if we can fix it
 [@@expect_failure]
 ```pulse
-fn read_at_offset_refine (a:array U32.t) (i:US.t) (#p:perm) (#s:Ghost.erased (Seq.seq U32.t))
+fn read_at_offset_refine_fail (a:array U32.t) (i:US.t) (#p:perm) (#s:Ghost.erased (Seq.seq U32.t))
    requires (A.pts_to a p s `star` pure (US.v i < A.length a))
    returns x: (x:U32.t { Seq.length s == A.length a /\
                          x == Seq.index s (US.v i)})
@@ -147,7 +96,7 @@ fn read_at_offset_refine (a:array U32.t) (i:US.t) (#p:perm) (#s:Ghost.erased (Se
       A.pts_to a p s
    )
 { 
-   let x = test_array_access a i;
+   let x = a.(i);
    (x <: (x:U32.t { Seq.length s == A.length a /\
                     US.v i < A.length a /\
                     x == Seq.index s (US.v i)}))
@@ -156,7 +105,7 @@ fn read_at_offset_refine (a:array U32.t) (i:US.t) (#p:perm) (#s:Ghost.erased (Se
 
 //But if we hoist the pure payload into a refinement, then it can be used for typing throughout the spec & body
 ```pulse
-fn read_at_offset_refine_post (a:array U32.t) (i:(i:US.t { US.v i < A.length a})) (#p:perm) (#s:Ghost.erased (Seq.seq U32.t))
+fn read_at_offset_refine (a:array U32.t) (i:(i:US.t { US.v i < A.length a})) (#p:perm) (#s:Ghost.erased (Seq.seq U32.t))
    requires (A.pts_to a p s)
    returns x: (x:U32.t { Seq.length s == A.length a /\
                          x == Seq.index s (US.v i)})
@@ -164,13 +113,14 @@ fn read_at_offset_refine_post (a:array U32.t) (i:(i:US.t { US.v i < A.length a})
       A.pts_to a p s
    )
 { 
-   let x = test_array_access a i;
-   x
-}
+   let x = a.(i);
+   (x <: (x:U32.t { Seq.length s == A.length a /\
+                         x == Seq.index s (US.v i)}))
+} 
 ```
 
 ```pulse
-fn read_at_offset_refine_post2 (a:array U32.t) (i:US.t) (#p:perm) (#s:Ghost.erased (Seq.seq U32.t))
+fn read_at_offset_refine2 (a:array U32.t) (i:US.t) (#p:perm) (#s:Ghost.erased (Seq.seq U32.t))
    requires (A.pts_to a p s `star` pure (US.v i < A.length a))
    returns x: (x:U32.t { Seq.length s == A.length a /\
                          US.v i < A.length a /\
@@ -179,8 +129,10 @@ fn read_at_offset_refine_post2 (a:array U32.t) (i:US.t) (#p:perm) (#s:Ghost.eras
       A.pts_to a p s
    )
 { 
-   let x = test_array_access a i;
-   x
+   let x = a.(i);
+   (x <: (x:U32.t { Seq.length s == A.length a /\
+                    US.v i < A.length a /\
+                    x == Seq.index s (US.v i)}))
 } 
 ```
 
@@ -188,21 +140,88 @@ fn read_at_offset_refine_post2 (a:array U32.t) (i:US.t) (#p:perm) (#s:Ghost.eras
 fn write_at_offset (#t:Type0) (a:array t) (i:US.t) (v:t)
                    (#s:(s:Ghost.erased (Seq.seq t) {US.v i < Seq.length s}))
    requires (A.pts_to a full_perm s)
-   ensures (
-      A.pts_to a full_perm (Seq.upd s (US.v i) v)
-   )
+   ensures (A.pts_to a full_perm (Seq.upd s (US.v i) v))
 {
    (a.(i) <- v)
 }
 ```
 
+```pulse
+fn write_at_offset_refine_post (#t:Type0) (a:array t) (i:US.t) (v:t) (#s:Ghost.erased (Seq.seq t))
+   requires (A.pts_to a full_perm s `star`
+               pure (US.v i < Seq.length s))
+   returns a: (a:array t { US.v i < Seq.length s })
+   ensures (A.pts_to a full_perm (Seq.upd s (US.v i) v))
+{
+   (a.(i) <- v);
+   (a <: (a:array t { US.v i < Seq.length s }))
+}
+```
+
+```pulse
+fn write_then_read (#t:Type0) (a:array t) (i:US.t) (v:t)
+                   (#s:(s:Ghost.erased (Seq.seq t) {US.v i < Seq.length s}))
+   requires (A.pts_to a full_perm s `star`
+             pure (US.v i < Seq.length s))
+   returns x:t
+   ensures (
+      A.pts_to a full_perm (Seq.upd s (US.v i) v) `star`
+      pure (US.v i < Seq.length (Seq.upd s (US.v i) v) /\
+            x == Seq.index (Seq.upd s (US.v i) v) (US.v i))
+   )
+{
+   (a.(i) <- v);
+   let x = a.(i);
+   x
+} 
+```
+
+```pulse
+fn write_then_read_twice (#t:Type0) (a:array t) (i:US.t) (v1 v2:t)
+                         (#s:(s:Ghost.erased (Seq.seq t) {US.v i < Seq.length s}))
+   requires (A.pts_to a full_perm s `star`
+             pure (US.v i < Seq.length s))
+   returns x:t
+   ensures (
+      A.pts_to a full_perm (Seq.upd (Seq.upd s (US.v i) v1) (US.v i) v2) `star`
+      pure (US.v i < Seq.length (Seq.upd (Seq.upd s (US.v i) v1) (US.v i) v2) /\
+            x == Seq.index (Seq.upd (Seq.upd s (US.v i) v1) (US.v i) v2) (US.v i))
+   )
+{
+   let x1 = write_then_read a i v1;
+   let x2 = write_then_read a i v2;
+   x2
+} 
+```
+
+```pulse
+fn write_then_read_twice_neq (#t:Type0) (a:array t) (i:US.t) (v1 v2:t)
+                             (#s:(s:Ghost.erased (Seq.seq t) {US.v i < Seq.length s}))
+   requires (A.pts_to a full_perm s `star`
+             pure (US.v i < Seq.length s /\
+                  ~(v1 == v2)))
+   returns p: t&t
+   ensures (
+      A.pts_to a full_perm (Seq.upd (Seq.upd s (US.v i) v1) (US.v i) v2) `star`
+      pure (US.v i < Seq.length (Seq.upd (Seq.upd s (US.v i) v1) (US.v i) v2) /\
+            snd p == Seq.index (Seq.upd (Seq.upd s (US.v i) v1) (US.v i) v2) (US.v i) /\
+            ~(fst p == snd p))
+   )
+{
+   let x1 = write_then_read a i v1;
+   let x2 = write_then_read a i v2;
+   (x1,x2)
+} 
+```
+
 let sorted (s0 s:Seq.seq U32.t) =
    (forall (i:nat). i < Seq.length s - 1 ==> U32.v (Seq.index s i) <= U32.v (Seq.index s (i + 1))) /\
-   (forall (i:nat). i < Seq.length s0 ==> (exists (j:nat). j < Seq.length s /\ U32.v (Seq.index s0 i) == U32.v (Seq.index s j)))
+   (forall (i:nat). i < Seq.length s0 ==> (exists (j:nat). j < Seq.length s /\ U32.v (Seq.index s0 i) == U32.v (Seq.index s j))) /\
+   (Seq.length s0 = Seq.length s)
 
 
 open FStar.UInt32
-#push-options "--query_stats"
+// #push-options "--query_stats"
 
 ```pulse
 fn sort3 (a:array U32.t)
@@ -310,3 +329,97 @@ fn sort3_alt (a:array U32.t)
    ()
 }
 ```
+
+```pulse
+fn swap (r1 r2:ref U32.t)
+        (#n1 #n2:erased U32.t)
+  requires 
+     (pts_to r1 full_perm n1 `star`
+      pts_to r2 full_perm n2)
+  ensures
+     (pts_to r1 full_perm n2 `star`
+      pts_to r2 full_perm n1)
+{
+  let x = !r1;
+  let y = !r2;
+  r1 := y;
+  r2 := x
+}
+```
+
+let my_sorted (s:Seq.seq U32.t) =
+  forall (i:nat). i < Seq.length s - 1 ==> U32.v (Seq.index s i) <= U32.v (Seq.index s (i + 1))
+
+```pulse 
+fn insert_into_sorted (a:array U32.t) (l:(l:nat{A.length a = l})) (#s:Ghost.erased (Seq.seq U32.t))
+	requires (A.pts_to a full_perm s `star`
+						pure (A.length a = Seq.length s /\
+									// my_sorted (Seq.slice s 0 (A.length a - 1))))
+									my_sorted (Seq.slice s 0 (A.length a))))
+	returns a:array U32.t
+	ensures 
+		exists s'. (
+				A.pts_to a full_perm s' `star`
+        pure (my_sorted s')
+    )
+{
+	let mut j = l - 1;
+	// while (let vj = !j; (vj > 0 /\ a.(vj-1) > a.(vj)))
+	while (let vj = !j; (vj > 0))
+	invariant b. exists vj. (
+      pts_to j full_perm vj `star`
+      pure (0 <= vj /\
+            vj <= l - 1 /\
+            my_sorted (Seq.slice s (vj-1) l) /\
+            // b == (vj > 0 /\ a.(vj-1) > a.(vj)))
+            b == (vj > 0))
+  )
+  {
+    let vj = !j;
+    // swap a.(vj-1) a.(vj);
+    j := vj - 1
+  };
+  a
+}
+```
+
+(*
+```pulse
+fn isort (a:array U32.t) (#s:Ghost.erased (Seq.seq U32.t))
+   requires (A.pts_to a full_perm s)
+   ensures 
+      exists s'. (
+         A.pts_to a full_perm s' `star`
+         pure (sorted s s')
+      )
+{
+   let mut i = 1;
+   while (let vi = !i; (vi < A.length a))
+   invariant b. exists vi s'. (
+      pts_to i full_perm vi `star`
+      A.pts_to a full_perm s' `star`
+      pure (1 <= vi /\
+            vi <= A.length a /\
+            sorted (Seq.slice s 0 vi) s' /\
+            b == (vi < A.length a))
+   )
+   {
+      let mut j = !i;
+      while (let vj = !j; (vj > 0 /\ a.(vj-1) > a.(vj)))
+      invariant b. exists vj. (
+         pts_to j full_perm vj `star`
+         pure (0 <= vj /\
+               vj <= i /\
+               b == (vj > 0 /\ a.(vj-1) > a.(vj)))
+      )
+      {
+         let vj = !j;
+         swap a.(vj-1) a.(vj);
+         j := vj - 1
+      };
+      let vi = !i;
+      i := vi + 1
+   };
+}
+```
+*)
