share/steel/examples/pulse/Factorial.fst
@@ -1,0 +1,43 @@
+module Factorial
+module T = FStar.Tactics
+module PM = Pulse.Main
+open Steel.ST.Util 
+open Steel.ST.Reference
+open Steel.FractionalPermission
+open FStar.Ghost
+module U32 = FStar.UInt32
+open Pulse.Steel.Wrapper
+open FStar.Mul
+
+let rec fac (n:nat) : nat =
+    if n = 0 then 1
+    else n * fac (n-1)
+
+```pulse
+fn fac_imp (n:pos)
+  requires emp
+  returns r:int
+  ensures pure (r == fac n)
+{
+  let mut acc = 1;
+  let mut ctr = 1;
+  while (let vctr = !ctr; (vctr < n))
+  invariant b . exists vacc vctr. (
+    pts_to acc full_perm vacc `star`
+    pts_to ctr full_perm vctr `star`
+    pure (1 <= vctr /\
+          vctr <= n /\
+          vacc == fac vctr /\
+          b == (vctr < n))
+  )
+  {
+    let vc = !ctr;
+    let va = !acc;
+    ctr := vc + 1;
+    acc := (vc + 1) * va;
+    ()
+  };
+  let r = !acc;
+  r
+}
+```
